sha3/proof/TopLevel.ec
@@ -1,7 +1,7 @@
 (*------------------------- Sponge Construction ------------------------*)
 
-require import Pair Int IntDiv Real List Option NewFMap.
-require import Common.
+require import Pair Int IntDiv Real List Option FSet NewFMap DBool.
+require import Fun Common.
 require (*--*) IRO Block.
 
 (*------------------------- Indifferentiability ------------------------*)
@@ -21,7 +21,8 @@ clone include Indifferentiability with
 clone import IRO as BIRO with
   type from <- bool list,
   type to   <- bool,
-  op valid  <- valid_toplevel.
+  op valid  <- valid_toplevel,
+  op dto    <- dbool.
 
 (*------------------------- Sponge Construction ------------------------*)
 
@@ -53,8 +54,6 @@ module Sponge (P : DPRIMITIVE) : FUNCTIONALITY, CONSTRUCTION(P) = {
 (*------------- Simulator and Distinguisher Constructions --------------*)
 
 module LowerFun (F : DFUNCTIONALITY) : Block.DFUNCTIONALITY = {
-  proc init() = {}
-
   proc f(xs : block list, n : int) = {
     var cs, ds : bool list;
     var obs : bool list option;
@@ -63,15 +62,13 @@ module LowerFun (F : DFUNCTIONALITY) : Block.DFUNCTIONALITY = {
     obs <- unpad_blocks xs;
     if (obs <> None) {
       cs <@ F.f(oget obs, n * r); (* size cs = n * r *)
-      ys <- bits2blocks cs;
+      ys <- bits2blocks cs; (* size ys = n *)
     }
     return ys;
   }
 }.
 
 module RaiseFun (F : Block.DFUNCTIONALITY) : DFUNCTIONALITY = {
-  proc init() = {}
-
   proc f(bs : bool list, n : int) = {
     var xs;
 
@@ -91,7 +88,175 @@ section.
 declare module BlockSim  : Block.SIMULATOR{IRO, Block.BIRO.IRO}.
 declare module Dist : DISTINGUISHER{Perm, BlockSim, IRO, Block.BIRO.IRO}.
 
-lemma Sponge_Raise_Block_Sponge_f :
+module type BLOCK_IRO_BITS = {
+  proc init() : unit
+  proc g(x : block list, n : int) : bool list
+  proc f(x : block list, n : int) : block list
+}.
+
+module type BLOCK_IRO_BITS_DIST(BIROB : BLOCK_IRO_BITS) = {
+  proc distinguish(): bool 
+}.
+
+local module BlockIROBitsEager : BLOCK_IRO_BITS, Block.BIRO.IRO = {
+  var mp : (block list * int, bool) fmap
+
+  proc init() : unit = {
+    mp <- map0;
+  }
+
+  proc fill_in(xs, i) = {
+    if (! mem (dom mp) (xs, i)) {
+      mp.[(xs, i)] <$ dbool;
+    }
+    return oget mp.[(xs, i)];
+  }
+
+  proc g(xs, n) = {
+    var b, bs;
+    var m <- ((n + r - 1) %/ r) * r;
+    var i <- 0;
+
+    bs <- [];
+    if (valid_block xs) {
+      while (i < n) {
+        b <@ fill_in(xs, i);
+        bs <- rcons bs b;
+        i <- i + 1;
+      }
+      while (i < m) {  (* eager part *)
+        fill_in(xs, i);
+        i <- i + 1;
+      }
+    }
+    return bs;
+  }
+
+  proc f(xs, n) = {
+    var bs, ys;
+    bs <@ g(xs, n * r);
+    ys <- bits2blocks bs;
+    return ys;
+  }
+}.
+
+local module BlockIROBitsLazy : BLOCK_IRO_BITS, Block.BIRO.IRO = {
+  var mp : (block list * int, bool) fmap
+
+  proc init() : unit = {
+    mp <- map0;
+  }
+
+  proc fill_in(xs, i) = {
+    if (! mem (dom mp) (xs, i)) {
+      mp.[(xs, i)] <$ dbool;
+    }
+    return oget mp.[(xs, i)];
+  }
+
+  proc g(xs, n) = {
+    var b, bs;
+    var i <- 0;
+
+    bs <- [];
+    if (valid_block xs) {
+      while (i < n) {
+        b <@ fill_in(xs, i);
+        bs <- rcons bs b;
+        i <- i + 1;
+      }
+    }
+    return bs;
+  }
+
+  proc f(xs, n) = {
+    var bs, ys;
+    bs <@ g(xs, n * r);
+    ys <- bits2blocks bs;
+    return ys;
+  }
+}.
+
+local module RaiseBIROBLazy (F : BLOCK_IRO_BITS) : FUNCTIONALITY = {
+  proc init() = {
+    F.init();
+  }
+
+  proc f(bs : bool list, n : int) = {
+    var cs;
+
+    cs <@ F.g(pad2blocks bs, n);
+    return take n cs;
+  }
+}.
+
+pred LazyInvar
+     (mp1 : (bool list * int, bool) fmap,
+      mp2 : (block list * int, bool) fmap) =
+  (forall (bs : bool list, n : int),
+   mem (dom mp1) (bs, n) <=> mem (dom mp2) (pad2blocks bs, n)) /\
+  (forall (xs : block list, n),
+   mem (dom mp2) (xs, n) => valid_block xs) /\
+  (forall (bs : bool list, n : int),
+   mem (dom mp1) (bs, n) =>
+   oget mp1.[(bs, n)] = oget mp2.[(pad2blocks bs, n)]).
+
+local lemma LowerFun_IRO_BlockIROBitsLazy_f :
+  equiv[LowerFun(IRO).f ~ BlockIROBitsLazy.f :
+        ={xs, n} /\ LazyInvar IRO.mp{1} BlockIROBitsLazy.mp{2} ==>
+        ={res} /\ LazyInvar IRO.mp{1} BlockIROBitsLazy.mp{2}].
+proof.
+proc=> /=; inline BlockIROBitsLazy.g.
+seq 0 1 :
+  (={n} /\ xs{1} = xs0{2} /\
+   LazyInvar IRO.mp{1} BlockIROBitsLazy.mp{2}); first auto.
+case (valid_block xs{1}).
+rcondt{1} 3; first auto. rcondt{2} 4; first auto.
+inline *. rcondt{1} 7; first auto.
+seq 6 3 : 
+  (={n, n0} /\ xs{1} = xs0{2} /\ n0{1} = n{1} * r /\
+   LazyInvar IRO.mp{1} BlockIROBitsLazy.mp{2} /\
+   valid_block xs{1} /\ pad2blocks x{1} = xs0{2}).
+auto; progress; have {2}<- /# := unpadBlocksK xs0{2}.
+admit.
+rcondf{1} 3; first auto. rcondf{2} 4; first auto.
+auto; progress; by rewrite bits2blocks_nil.
+qed.
+
+(* TODO:
+ 
+ IRO.f ~ RaiseBIROBLazy(BlockIROBitsLazy).f *)
+
+(* TODO:
+BlockIROBitsEager.f ~ Block.BIRO.IRO.f
+
+BlockIROBitsEager.fi ~ Block.BIRO.IRO.fi
+
+RaiseFun(BlockIROBitsEager).f ~ RaiseFun(Block.BIRO.IRO).f
+*)
+
+local lemma BlockIROBitsEager (D <: BLOCK_IRO_BITS_DIST) :
+  equiv[D(BlockIROBitsEager).distinguish ~ D(BlockIROBitsLazy).distinguish : 
+        ={glob D} /\ BlockIROBitsEager.mp{1} = BlockIROBitsLazy.mp{2} ==>
+        ={glob D}].
+proof.
+admit.
+qed.
+
+pred BlockIROBits_Eager_Invar
+     (mp1 : (block list * int, block) fmap,
+      mp2 : (block list * int, bool) fmap) =
+  (forall (xs : block list, i : int),
+   mem (dom mp1) (xs, i) =>
+   0 <= i /\
+   (forall (j : int), 0 <= j < i => mem (dom mp1) (xs, j)) /\
+   (forall (j : int), i * r <= j < (i + 1) * r =>
+    mp2.[(xs, j)] = Some(nth false (w2bits(oget mp1.[(xs, i)])) j))) /\
+  (forall (xs : block list, j : int),
+   mem (dom mp2) (xs, j) =>
+   0 <= j /\ mem (dom mp1) (xs, j %/ r)).
+
+local lemma Sponge_Raise_Block_Sponge_f :
   equiv[Sponge(Perm).f ~ RaiseFun(Block.Sponge(Perm)).f :
         ={bs, n, glob Perm} ==> ={res, glob Perm}].
 proof.
@@ -118,7 +283,7 @@ auto; progress; by rewrite -cats1 blocks2bits_cat blocks2bits_sing.
 auto.
 qed.
 
-lemma RealIndif &m :
+local lemma RealIndif &m :
   Pr[RealIndif(Sponge, Perm, Dist).main() @ &m: res] =
   Pr[Block.RealIndif
      (Block.Sponge, Perm, LowerDist(Dist)).main() @ &m : res].
@@ -130,34 +295,79 @@ conseq Sponge_Raise_Block_Sponge_f=> //.
 auto.
 qed.
 
-lemma IdealDist &1 &2 (a : bool) :
-  (glob Dist){1} = (glob Dist){2} => (glob BlockSim){1} = (glob BlockSim){2} =>
-  IRO.mp{1} = NewFMap.map0 => Block.BIRO.IRO.mp{2} = NewFMap.map0 =>
-  Pr[Dist(IRO, BlockSim(LowerFun(IRO))).distinguish() @ &1 : a = res] =
-  Pr[Dist(RaiseFun(Block.BIRO.IRO),
-          BlockSim(Block.BIRO.IRO)).distinguish() @ &2 : a = res].
+local lemma IdealIndifIROLazy &m :
+  Pr[IdealIndif(IRO, RaiseSim(BlockSim), Dist).main() @ &m : res] =
+  Pr[Experiment
+     (RaiseBIROBLazy(BlockIROBitsLazy), BlockSim(BlockIROBitsLazy),
+      Dist).main() @ &m : res].
 proof.
+byequiv=> //; proc.
+seq 2 2 :
+  (={glob Dist, glob BlockSim} /\ IRO.mp{1} = NewFMap.map0 /\
+   BlockIROBitsLazy.mp{2} = NewFMap.map0).
+inline *; wp; call (_ : true); auto.
+call
+  (_ :
+  ={glob Dist, glob BlockSim} /\
+  IRO.mp{1} = map0 /\ BlockIROBitsLazy.mp{2} = map0 ==>
+  ={res}).
+proc (={glob BlockSim}).
+smt.
+smt.
+admit.
+admit.
+admit.
+auto.
+qed.
+
+local lemma IdealIndifLazy &m :
+  Pr[Experiment
+     (RaiseBIROBLazy(BlockIROBitsLazy), BlockSim(BlockIROBitsLazy),
+      Dist).main() @ &m : res] =
+  Pr[Block.IdealIndif
+     (BlockIROBitsEager, BlockSim, LowerDist(Dist)).main() @ &m : res].
+proof.
+byequiv=> //; proc.
+seq 2 2 :
+  (={glob Dist, glob BlockSim} /\ BlockIROBitsLazy.mp{1} = NewFMap.map0 /\
+   BlockIROBitsEager.mp{2} = NewFMap.map0).
+inline *; wp; call (_ : true); auto.
+(* reduction to BlockIROBitsEager *)
 admit.
 qed.
 
-lemma IdealIndif &m :
-  Pr[IdealIndif(IRO, RaiseSim(BlockSim), Dist).main() @ &m : res] =
+local lemma IdealIndifEager &m :
+  Pr[Block.IdealIndif
+     (BlockIROBitsEager, BlockSim, LowerDist(Dist)).main() @ &m : res] =
   Pr[Block.IdealIndif
      (Block.BIRO.IRO, BlockSim, LowerDist(Dist)).main () @ &m : res].
 proof.
 byequiv=> //; proc.
 seq 2 2 :
-  (={glob Dist, glob BlockSim} /\ IRO.mp{1} = NewFMap.map0 /\
+  (={glob Dist, glob BlockSim} /\ BlockIROBitsEager.mp{1} = NewFMap.map0 /\
    Block.BIRO.IRO.mp{2} = NewFMap.map0).
 inline *; wp; call (_ : true); auto.
 call
   (_ :
   ={glob Dist, glob BlockSim} /\
-  IRO.mp{1} = map0 /\ Block.BIRO.IRO.mp{2} = map0 ==>
+  BlockIROBitsEager.mp{1} = map0 /\ Block.BIRO.IRO.mp{2} = map0 ==>
   ={res}).
-bypr res{1} res{2}=> //; progress.
-apply (IdealDist &1 &2 a)=> //.
+proc (={glob BlockSim}).
+smt.
+smt.
+proc (true); first 2 smt.
+admit.
+admit.
+admit.
 auto.
+qed.
+
+local lemma IdealIndif &m :
+  Pr[IdealIndif(IRO, RaiseSim(BlockSim), Dist).main() @ &m : res] =
+  Pr[Block.IdealIndif
+     (Block.BIRO.IRO, BlockSim, LowerDist(Dist)).main () @ &m : res].
+proof.
+by rewrite (IdealIndifIROLazy &m) (IdealIndifLazy &m) (IdealIndifEager &m).
 qed.
 
 lemma Conclusion' &m :
